platform/cito/LayoutHints2.v
@@ -1,7 +1,7 @@
 Set Implicit Arguments.
 
 Require Import ADT.
-Require Import RepInv.
+Require Import RepInv WordMap.
 
 Module Make (Import E : ADT) (Import M : RepInv E).
 
@@ -14,8 +14,443 @@ Module Make (Import E : ADT) (Import M : RepInv E).
 
     Definition heap_to_split h (_ : list (W * ArgIn)) := is_heap h.
 
+    Lemma starL_in : forall A P x (ls : list A),
+      NoDup ls
+      -> In x ls
+      -> exists ls', (P x * Bags.starL P ls' ===> Bags.starL P ls)
+        /\ NoDup ls'
+        /\ (forall y, In y ls' <-> y <> x /\ In y ls).
+      induction 1; simpl; intuition subst.
+
+      eexists; intuition idtac.
+      apply Himp_refl.
+      auto.
+      congruence.
+      tauto.
+      congruence.
+      auto.
+
+      destruct H1; intuition.
+      exists (x0 :: x1); intuition idtac.
+      simpl.
+      eapply Himp_trans; [ | apply Himp_star_frame; [
+        apply Himp_refl | apply H3 ] ].
+      generalize dependent (Bags.starL P); intros.
+      sepLemma.
+      constructor; auto.
+      intro.
+      apply H5 in H4.
+      tauto.
+      subst; simpl in *; intuition subst.
+      auto.
+      apply H5 in H6; intuition.
+      simpl in *; intuition subst.
+      apply H5 in H6; intuition.
+      subst; simpl; tauto.
+      right; apply H5.
+      auto.
+    Qed.
+
+    Lemma starL_out : forall A P x (ls : list A),
+      NoDup ls
+      -> In x ls
+      -> exists ls', (Bags.starL P ls ===> P x * Bags.starL P ls')
+        /\ NoDup ls'
+        /\ (forall y, In y ls' <-> y <> x /\ In y ls).
+      induction 1; simpl; intuition subst.
+
+      eexists; intuition idtac.
+      apply Himp_refl.
+      auto.
+      congruence.
+      tauto.
+      congruence.
+      auto.
+
+      destruct H1; intuition.
+      exists (x0 :: x1); intuition idtac.
+      simpl.
+      eapply Himp_trans; [ apply Himp_star_frame; [
+        apply Himp_refl | apply H3 ] | ].
+      generalize dependent (Bags.starL P); intros.
+      sepLemma.
+      constructor; auto.
+      intro.
+      apply H5 in H4.
+      tauto.
+      subst; simpl in *; intuition subst.
+      auto.
+      apply H5 in H6; intuition.
+      simpl in *; intuition subst.
+      apply H5 in H6; intuition.
+      subst; simpl; tauto.
+      right; apply H5.
+      auto.
+    Qed.
+
+    Lemma starL_permute : forall A P (ls1 : list A),
+      NoDup ls1
+      -> forall ls2, NoDup ls2
+        -> (forall x, In x ls1 <-> In x ls2)
+        -> Bags.starL P ls1 ===> Bags.starL P ls2.
+      induction 1.
+
+      inversion_clear 1; simpl; intros.
+      apply Himp_refl.
+      exfalso; eapply H; eauto.
+
+      intros.
+      eapply starL_in in H1.
+      Focus 2.
+      apply H2.
+      simpl; eauto.
+
+      destruct H1; intuition.
+      simpl.
+      eapply Himp_trans; [ | apply H3 ].
+      apply Himp_star_frame; try apply Himp_refl.
+      apply IHNoDup; auto.
+      intuition.
+      simpl in *.
+      apply H5; intuition.
+      apply H2; auto.
+      apply H5 in H4; intuition.
+      simpl in *.
+      apply H2 in H7.
+      intuition.
+    Qed.
+
+    Hint Constructors NoDup.
+
+    Theorem In_InA : forall A x ls,
+      In x ls -> SetoidList.InA (WordMap.eq_key (elt:=A)) x ls.
+      induction ls; simpl; intuition.
+    Qed.
+
+    Theorem NoDupA_NoDup : forall A ls,
+      SetoidList.NoDupA (WordMap.eq_key (elt:=A)) ls -> NoDup ls.
+      induction 1; eauto.
+      constructor; auto.
+      intro; apply H.
+      eauto using In_InA.
+    Qed.
+
+    Theorem In_InA' : forall A x ls,
+      In x ls -> SetoidList.InA (WordMap.eq_key_elt (elt:=A)) x ls.
+      induction ls; simpl; intuition.
+      subst; constructor; hnf; auto.
+    Qed.
+
+    Theorem InA_In : forall A x ls,
+      SetoidList.InA (WordMap.eq_key_elt (elt:=A)) x ls -> In x ls.
+      induction 1; simpl; intuition idtac.
+      destruct x, y; simpl in *.
+      hnf in H; simpl in *; intuition subst.
+      tauto.
+    Qed.
+
+    Lemma split_heap' : forall pairs h, good_inputs h pairs -> heap_to_split h pairs ===> let h1 := make_heap pairs in is_heap h1 * is_heap (heap_diff h h1).
+      unfold heap_to_split; induction pairs; simpl; intros.
+
+      unfold heap_diff, heap_empty.
+      eapply Himp_trans; [ | apply Himp_star_Emp' ].
+      unfold is_heap, heap_elements.
+      apply starL_permute.
+      
+      apply NoDupA_NoDup.
+      apply WordMap.elements_3w.
+
+      apply NoDupA_NoDup.
+      apply WordMap.elements_3w.
+
+      intuition.
+      apply In_InA' in H0.
+      apply InA_In.
+      apply WordMap.elements_1.
+      apply WordMap.elements_2 in H0.
+      apply Properties.diff_mapsto_iff.
+      intuition.
+      destruct H1.
+      eapply WordMap.empty_1; eauto.
+      apply In_InA' in H0.
+      apply WordMap.elements_2 in H0.
+      apply Properties.diff_mapsto_iff in H0.
+      intuition.
+      apply InA_In.
+      apply WordMap.elements_1; auto.
+
+      unfold is_heap, heap_elements.
+      destruct H.
+      inversion_clear H.
+      hnf in H1.
+      hnf in H0.
+      case_eq (snd a); intros.
+      rewrite H in *; subst.
+      unfold make_heap; simpl.
+      unfold store_pair at 2 4.
+      unfold ArgIn, Semantics.ArgIn.
+      unfold WordMap.key in H.
+      rewrite H.
+      apply IHpairs.
+      split; auto.
+      hnf.
+      simpl in H0.
+      unfold ArgIn, Semantics.ArgIn in H0.
+      rewrite H in H0.
+      auto.
+
+      rewrite H in H1.
+      generalize H1; intro Ho.
+      apply WordMap.find_2 in Ho.
+      apply WordMap.elements_1 in Ho.
+      apply InA_In in Ho.
+      eapply starL_out in Ho.
+      destruct Ho; intuition.
+      eapply Himp_trans; [ apply H4 | ].
+      clear H4; simpl.
+      2: apply NoDupA_NoDup; apply WordMap.elements_3w.
+      assert (In (fst a, a0) (WordMap.elements (elt:=elt) (make_heap (a :: pairs)))).
+      unfold make_heap; simpl.
+      
+      Lemma preserve_store : forall k v pairs h,
+        List.Forall (fun p => match snd p with
+                                | inl _ => True
+                                | inr _ => ~WordMap.In (fst p) h
+                              end) pairs
+        -> NoDup (map fst (filter (fun p => Semantics.is_adt (snd p)) pairs))
+        -> WordMap.MapsTo k v h
+        -> WordMap.MapsTo k v (fold_left store_pair pairs h).
+        induction pairs; simpl in *; intuition.
+        inversion_clear H; simpl in *.
+        apply IHpairs; auto.
+
+        simpl in *.
+        inversion_clear H; simpl in *.
+        inversion_clear H0.
+        apply IHpairs; auto.
+        unfold store_pair; simpl.
+        eapply Forall_forall; intros.
+        case_eq (snd x); intuition idtac.
+        eapply Forall_forall in H3; [ | eassumption ].
+        unfold heap_upd in H6.
+        rewrite H5 in *.
+        apply Properties.F.add_in_iff in H6; intuition subst.
+        apply H.
+        apply in_map.
+        apply filter_In; intuition idtac.
+        unfold Semantics.is_adt.
+        unfold WordMap.key, Semantics.ArgIn in *.
+        rewrite H5; reflexivity.
+        unfold store_pair; simpl.
+        unfold heap_upd.
+        apply Properties.F.add_mapsto_iff.
+        right; intuition subst.
+        apply H2.
+        exists v; auto.
+      Qed.
+
+      apply InA_In.
+      apply Properties.F.elements_mapsto_iff.
+      simpl in H0.
+      unfold Semantics.is_adt in H0.
+      unfold WordMap.key, Semantics.ArgIn in *.
+      rewrite H in *; simpl in *.
+      inversion_clear H0.
+      apply preserve_store; auto.
+      apply Forall_forall; intros.
+      case_eq (snd x0); intuition idtac.
+      unfold store_pair in H8.
+      unfold WordMap.key, ArgIn, Semantics.ArgIn in *.
+      rewrite H in H8.
+      unfold heap_upd in H8.
+      eapply Properties.F.add_in_iff in H8; intuition idtac.
+      2: destruct H9; eapply WordMap.empty_1; eauto.
+      destruct a; simpl in *; subst.
+      destruct x0; simpl in *; subst.
+      
+      Lemma keep_key : forall w a1 pairs,
+        In (w, inr a1) pairs
+        -> In w (map fst (filter
+          (fun p : W * (W + ADTValue) =>
+            match snd p with
+              | inl _ => false
+              | inr _ => true
+            end) pairs)).
+        induction pairs; simpl; intuition (subst; simpl in *); intuition idtac.
+      Qed.
+
+      eauto using keep_key.
+      unfold store_pair.
+      unfold WordMap.key, ArgIn, Semantics.ArgIn in *.
+      rewrite H.
+      unfold heap_upd.
+      apply WordMap.add_1; auto.
+
+      simpl in *.
+      destruct a; simpl in *; subst; simpl in *.
+      inversion_clear H0.
+      eapply Himp_trans; [ | apply Himp_star_frame; [ apply starL_permute | apply Himp_refl ] ].
+      instantiate (1 := (k, a0) :: heap_elements (make_heap pairs)).
+      Focus 2.
+      constructor.
+      intro.
+      unfold heap_elements, make_heap in H0.
+      apply In_InA' in H0.
+      apply WordMap.elements_2 in H0.
+
+      Lemma store_keys : forall k v pairs h,
+        WordMap.MapsTo k v (fold_left store_pair pairs h)
+        -> In (k, inr v) pairs \/ WordMap.MapsTo k v h.
+        induction pairs; simpl; intuition idtac.
+        apply IHpairs in H; intuition idtac.
+        unfold store_pair in H0; simpl in H0.
+        destruct b; auto.
+        unfold heap_upd in H0.
+        apply Properties.F.add_mapsto_iff in H0; intuition subst; auto.
+      Qed.
+
+      apply store_keys in H0; intuition idtac.
+      apply H.
+      change k with (fst (k, @inr W _ a0)).
+      apply in_map; apply filter_In; tauto.
+      eapply WordMap.empty_1; eauto.
+      apply NoDupA_NoDup; apply WordMap.elements_3w.
+      2: apply NoDupA_NoDup; apply WordMap.elements_3w.
+      Focus 2.
+      simpl.
+      split.
+      destruct 1; subst.
+      auto.
+      unfold heap_elements in H0.
+      
+      Lemma store_keys'' : forall k v pairs h,
+        WordMap.MapsTo k v h
+        -> ~In k (map fst (filter (fun p => Semantics.is_adt (snd p)) pairs))
+        -> WordMap.MapsTo k v (fold_left store_pair pairs h).
+        induction pairs; simpl; intuition (try discriminate; eauto);
+          unfold Semantics.is_adt in *; simpl in *.
+
+        destruct b; auto.
+        simpl in *; intuition subst.
+        apply IHpairs; auto.
+        unfold store_pair, heap_upd; simpl.
+        apply Properties.F.add_mapsto_iff; auto.
+      Qed.
+
+      Lemma store_keys' : forall k v pairs h,
+        In (k, inr v) pairs
+        -> NoDup (map fst (filter (fun p => Semantics.is_adt (snd p)) pairs))
+        -> WordMap.MapsTo k v (fold_left store_pair pairs h).
+        induction pairs; simpl; intuition (try discriminate; eauto);
+          unfold Semantics.is_adt in *; simpl in *.
+
+        injection H1; clear H1; intros; subst.
+        inversion_clear H0.
+        apply store_keys''; auto.
+        unfold store_pair, heap_upd; simpl.
+        apply Properties.F.add_mapsto_iff; auto.
+
+        inversion_clear H0; eauto.
+      Qed.
+
+      apply InA_In.
+      destruct x0.
+      apply WordMap.elements_1.
+      unfold make_heap; simpl.
+      apply store_keys'; auto.
+      apply In_InA' in H0.
+      apply WordMap.elements_2 in H0.
+      apply store_keys in H0; intuition idtac.
+      exfalso; eapply WordMap.empty_1; eauto.
+
+      intro.
+      apply In_InA' in H0.
+      destruct x0.
+      apply WordMap.elements_2 in H0.
+      unfold make_heap in H0; simpl in H0.
+      apply store_keys in H0.
+      intuition idtac.
+      right.
+      apply InA_In.
+      apply WordMap.elements_1.
+      apply store_keys'; auto.
+      unfold store_pair in H7; simpl in H7.
+      apply Properties.F.add_mapsto_iff in H7; intuition subst.
+      auto.
+      exfalso; eapply WordMap.empty_1; eauto.      
+      
+      simpl.
+      eapply Himp_trans; [ | apply Himp_star_assoc' ].
+      apply Himp_star_frame; try apply Himp_refl.
+      eapply Himp_trans; [ apply starL_permute | ].
+      auto.
+      instantiate (1 := WordMap.elements (WordMap.remove k h)).
+      apply NoDupA_NoDup; apply WordMap.elements_3w.
+      split; intro.
+      apply InA_In.
+      destruct x0.
+      apply WordMap.elements_1.
+      apply Properties.F.remove_mapsto_iff.
+      apply H6 in H0.
+      destruct H0; split; auto.
+      2: apply WordMap.elements_2; apply In_InA'; auto.
+      apply In_InA' in H7; apply WordMap.elements_2 in H7.
+      apply WordMap.find_1 in H7.
+      congruence.
+      apply In_InA' in H0.
+      destruct x0; apply WordMap.elements_2 in H0.
+      apply Properties.F.remove_mapsto_iff in H0.
+      apply H6; intuition (try congruence).
+      apply InA_In; apply WordMap.elements_1; auto.
+
+      eapply Himp_trans; [ apply IHpairs | ]; clear IHpairs.
+      split; auto.
+      apply Forall_forall; intros.
+      eapply Forall_forall in H2; [ | apply H0 ].
+      hnf in H2; hnf.
+      destruct x0; simpl in *.
+      destruct s; auto.
+      apply WordMap.find_1.
+      apply Properties.F.remove_mapsto_iff.
+      apply WordMap.find_2 in H2.
+      intuition subst.
+      apply H.
+      change k0 with (@fst W (Semantics.ArgIn ADTValue) (k0, inr a)).
+      apply in_map.
+      apply filter_In; auto.
+
+      apply Himp_star_frame; try apply Himp_refl.
+      apply starL_permute; try (apply NoDupA_NoDup; apply WordMap.elements_3w); intros.
+      intuition; apply InA_In; apply WordMap.elements_1;
+        apply In_InA' in H0; apply WordMap.elements_2 in H0;
+          apply Properties.diff_mapsto_iff; apply Properties.diff_mapsto_iff in H0; intuition idtac.
+      apply Properties.F.remove_mapsto_iff in H7; tauto.
+      apply Properties.F.remove_mapsto_iff in H7; intuition subst.
+      destruct H0.
+      eapply store_keys in H0; intuition idtac.
+      simpl in *; intuition (try congruence).
+      apply H8.
+      eexists.
+      eapply store_keys'; eauto.
+      exfalso; eapply WordMap.empty_1; eauto.
+      apply Properties.F.remove_mapsto_iff; intuition subst.
+      apply H8.
+      eexists; eapply store_keys'; eauto.
+      simpl; eauto.
+      auto.
+      constructor; auto.
+      apply H8.
+      destruct H0.
+      eapply store_keys in H0; intuition idtac.
+      eexists.
+      eapply store_keys'.
+      simpl; eauto.
+      constructor; auto.
+      exfalso; eapply WordMap.empty_1; eauto.
+    Qed.
+
     Lemma split_heap : forall h pairs, good_inputs h pairs -> heap_to_split h pairs ===> let h1 := make_heap pairs in is_heap h1 * is_heap (heap_diff h h1).
-      admit.
+      eauto using split_heap'.
     Qed.
 
     Definition hints_split_heap : TacPackage.
